Solving for the complamentary cumulative distributions for continuous distributions. The formula used for solving for the complamentary cumulative distribution is,
\[
  P_\leq (A)
  =
  \int_{p^{-1}(A^{-\gamma})}^\infty
    p(x)dx
  =
  p_\leq(p^{-1}(A^{-\gamma}))
 \addtag
\]

Here $p^{-1}$ represents the inverse function, so that is the first thing that needs to be found.

(a) Solving for
$P_\leq (A)$
from
$p(x) = cx^{ -(q+1) }$

\[
  p = cx^{ -(q+1) }
  \addtag
\]

\[
  x = cp'^{ -(q+1) }
  \addtag
\]

\[
  x / c
  =
  p'^{ -(q+1) }
  \addtag
\]

\[
  p'
  =
  (x / c)^{-(\frac{1}{q + 1})}
  \addtag
\]

\[
  p'(A^{-\gamma})
  =
  (A^{-\gamma} / c)^{-(\frac{1}{q + 1})}
  \addtag
\]

\[
  P_\leq (A)
  =
  \int_{
    \frac{A^{-\gamma}}{c}
      ^{-(\frac{1}{q + 1})}
    }^\infty
    cx^{ -(q+1) }
    dx
  \addtag
\]

\[
  =
  \left.
  -\frac{c}{q}
   x^{-q}
  \right|_{
    (A^{-\gamma} / c)^{-(\frac{1}{q + 1})}
  }^{
    \infty
  }
  \addtag
\]

\[
  =
  \left[
    0 -
    -\frac{c}{q}
    \left(
      (A^{-\gamma} / c)
        ^{-(\frac{1}{q + 1})}
    \right)^{-q}
  \right]
  \addtag
\]

\[
  =
  \frac{c}{q}
  \left(
    (A^{-\gamma} / c)^{-(\frac{1}{q + 1})}
  \right)^{-q}
  \addtag
\]

\[
  =
  \frac{c}{q}
  \left(
    \frac{A^{-\gamma}}{c}
  \right)
    ^{-(\frac{q}{q + 1})}
  \addtag
\]

\[
  =
  \frac{c}{q}
  \left(
    \frac{A^{-\gamma}}{c}
  \right)
    ^{-(1 + \frac{1}{q})}
  \addtag
\]

(b) Solving for
$P_\leq (A)$
from
$p(x) = ce^{-x}$ 

\[
  p = e^{-x}
  \addtag
\]

\[
  x = e^{-p'}
  \addtag
\]

\[
  ln(x) = -p'
  \addtag
\]

\[
  p' = -ln(x)
  \addtag
\]

\[
  p'(A^{-\gamma}) =
  -ln(A^{-\gamma})
  \addtag
\]

\[
  P_\leq (A)
  =
  \int_{-ln(A^{-\gamma})}^\infty
    ce^{-x}
    dx
  \addtag
\]

\[
  =
  \left.
    -ce^{-x}
  \right|_{-ln(A^{-\gamma})}^{\infty}
  \addtag
\]

\[
  =
  \left(
    0
      -
    -ce^{-(-ln(A^{-\gamma}))}
  \right)
  \addtag
\]

\[
  =
  ce^{ln(A^{-\gamma})}
  \addtag
\]

\[
  P_\leq (A)
  =
  cA^{-\gamma}
  \addtag
\]

(c) Solving for
$P_\leq (A)$
from
$p(x) = ce^{-x^2}$

\[
  p = ce^{-x^2}
  \addtag
\]

\[
  x = ce^{-p'^2}
  \addtag
\]

\[
  x = ce^{-p'^2}
  \addtag
\]

\[
  x / c
  =
  e^{-p'^2}
  \addtag
\]

\[
  ln(x / c)
  =
  -p'^2
  \addtag
\]

\[
  p'
  =
  (-ln(x / c))^{1/2}
  \addtag
\]

\[
  p'(A^{-\gamma})
  =
  (-ln(A^{-\gamma} / c))^{1/2}
  \addtag
\]

\[
  P_\leq (A)
  =
  \int_{
    (-ln(A^{-\gamma} / c))^{1/2}
  }^\infty
    ce^{-x^2}
    dx
  \addtag
\]